.

sf/Imp.v
@@ -1,19 +1,9 @@
 Require Import Coq.Arith.Arith.
+Require Import Coq.Strings.String.
 Require Import Maps.
+Require Import Coq.Logic.FunctionalExtensionality.
 
-Module ANum.
-
-Inductive aexp : Type :=
-ANum : nat -> aexp
-.
-
-Inductive bexp : Type :=
-BEq : aexp -> aexp -> bexp
-.
-
-Inductive aevalR : aexp -> nat -> Prop :=
-| E_ANum : forall (n:nat), aevalR (ANum n) n
-.
+Module MSkip.
 
 Definition state := total_map nat.
 
@@ -21,7 +11,148 @@ Inductive com : Type :=
 | CSkip : com
 .
 
-Inductive
+Inductive ceval : com -> state -> state -> Prop :=
+| E_Skip : forall s:state, ceval CSkip s s
+.
+
+Theorem ceval_deterministic : forall (c:com) (src:state) (dst1:state) (dst2:state),
+ceval c src dst1 -> ceval c src dst2 -> dst1 = dst2.
+intros c src dst1 dst2.
+intros h1 h2.
+inversion h1. subst s. subst dst1.
+subst c.
+inversion h2. subst s. subst dst2.
+reflexivity.
+Qed.
+
+Theorem nothing: forall (c:com) (src dst:state),
+ceval c src dst -> src = dst.
+intros c src dst.
+intro h. inversion h. reflexivity.
+Qed.
+
+End MSkip.
+
+Module MAssignment.
+
+Definition state := partial_map nat.
+
+Inductive com : Type :=
+| CSkip : com
+| CAss : string -> nat -> com
+.
+
+Inductive ceval : com -> state -> state -> Prop :=
+| E_Skip : forall s:state, ceval CSkip s s
+| E_Ass : forall (s:state) (id:string) (n:nat), ceval (CAss id n) s (update s id n)
+.
+
+Theorem alln : forall (n:nat) (src dst:state), exists (c:com), ceval c src dst -> exists id:string, dst id = Some n.
+intros n src dst.
+exists (CAss "A" n).
+intro h.
+exists "A"%string.
+inversion h. subst n0. subst id. subst s.
+unfold update.
+unfold t_update.
+rewrite beq_string_refl.
+reflexivity.
+Qed.
+
+Theorem state_different_single_variable : forall (src dst:state) (c:com),
+src=empty /\ ceval c src dst /\ src <> dst ->
+exists (id:string) (n:nat), dst id = Some n /\
+  forall (id':string) (n':nat), dst id' = Some n' -> n=n' /\ id=id'.
+Proof.
+intros src dst c.
+intros [empty [heval hneq]].
+inversion heval.
+subst c. subst s. subst src. contradiction.
+subst s. exists id. exists n.
+split.
+unfold update. unfold t_update. rewrite beq_string_refl. reflexivity.
+intros id' n'.
+intro update'.
+unfold update in update'.
+unfold t_update in update'.
+subst c.
+
+unfold beq_string in update'.
+destruct (string_dec id id').
+subst id'.
+inversion update'.
+subst n'.
+split;reflexivity.
+
+subst src. inversion update'.
+
+Qed.
 
 
-End ANum.
+End MAssignment.
+
+Module MSkipAndSeq.
+
+Definition state := partial_map nat.
+
+Inductive com : Type :=
+| CSkip : com
+| CSeq : com -> com -> com
+.
+
+Inductive ceval : com -> state -> state -> Prop :=
+| E_Skip : forall s:state, ceval CSkip s s
+| E_Seq : forall (src tmp dst:state) (c1 c2:com), ceval c1 src tmp -> ceval c2 tmp dst -> ceval (CSeq c1 c2) src dst
+.
+
+Theorem nothing : forall (src dst:state) (c:com), ceval c src dst -> src = dst.
+Proof.
+intros src dst c.
+generalize src dst.
+clear src dst.
+induction c.
+intros src dst heval. inversion heval. reflexivity.
+intros src dst heval.
+inversion heval.
+subst dst0 src0 c3 c0.
+rewrite <- (IHc2 tmp dst).
+rewrite <- (IHc1 src tmp).
+reflexivity. assumption. assumption.
+Qed.
+
+Theorem nothing2 : forall (s:state) (c:com), ceval c s s.
+Proof.
+intros s c. generalize s. clear s. induction c.
+intros;constructor.
+intro s.
+apply (E_Seq s s s). apply IHc1. apply IHc2.
+Qed.
+
+Theorem something_impossible : forall (src dst:state) (c:com), not (ceval c src dst /\ src <> dst).
+intros src dst c.
+intros [heval hneq].
+apply hneq.
+rewrite (nothing src dst c). reflexivity. assumption.
+Qed.
+
+Fixpoint contains_skip (c:com) : Prop :=
+match c with
+| CSkip => True
+| CSeq c1 c2 => (contains_skip c1) \/ (contains_skip c2)
+end.
+
+Theorem must_skip : forall (src dst:state) (c:com), ceval c src dst -> contains_skip c.
+intros src dst c.
+generalize dependent dst.
+generalize dependent src.
+induction c.
+simpl. trivial.
+intros src dst heval.
+simpl.
+inversion heval.
+subst dst0 src0 c3 c0.
+right. apply (IHc2 tmp dst). assumption.
+Qed.
+
+
+End MSkipAndSeq.
